# Chapter 2

## Exercise 1a

We have
$$
a\ ⋆\ b = ab + a + b \\
a, b \in \mathbb{R} \setminus \{-1\} \\
$$

Suppose that
$$
a\ ⋆\ b = -1
$$

Then,
$$
\begin{align*}
ab + a + b &= -1 \\
a(b+1) + b + 1 &= 0 \\
(a + 1)(b + 1) &= 0 \\
(a + 1) = 0 \quad &\text{or} \quad (b + 1) = 0 \\
a = -1 \quad &\text{or} \quad b = -1
\end{align*}
$$

Contradicts $a, b \in \mathbb{R} \setminus \{-1\}$. Thus, $a\ ⋆\ b \ne -1$. This proves the _closure_ property.

$$

\begin{align*}

a\ ⋆\ b = ab + a + b \\
a = b

\end{align*}
$$



